Proved the DFacade version without operational specs

platform/facade/CompileDFacade.v
@@ -26,16 +26,6 @@ Fixpoint compile (s : Stmt) : Facade.Stmt :=
         (Facade.Call x (Var fun_ptr_varname) args)
   end.
 
-Lemma compile_no_assign_to_args (spec : OperationalSpec) : is_disjoint (Facade.assigned (compile (Body spec))) (ArgVars spec) = true.
-  admit.
-Qed.
-
-Definition compile_op (spec : OperationalSpec) : Facade.OperationalSpec.
-  refine
-    (Facade.Build_OperationalSpec (ArgVars spec) (RetVar spec) (compile (Body spec)) (args_no_dup spec) (ret_not_in_args spec) _).
-  eapply compile_no_assign_to_args.
-Defined.
-
 Section ADTValue.
 
   Variable ADTValue : Type.
@@ -60,18 +50,12 @@ Section ADTValue.
 
   Arguments Facade.Operational {ADTValue} _.
 
-  Definition compile_spec (spec : FuncSpec) : FFuncSpec :=
-    match spec with
-      | Axiomatic s => Facade.Axiomatic s
-      | Operational s => Facade.Operational (compile_op s)
-    end.
-
   Definition fenv_impls_env (fenv : FEnv) (env : Env) :=
     forall lbl spec,
       find lbl env = Some spec ->
       exists w,
         Label2Word fenv lbl = Some w /\
-        Word2Spec fenv w = Some (compile_spec spec).
+        Word2Spec fenv w = Some (Axiomatic spec).
     
   Require Import GeneralTactics4.
   Require Import GeneralTactics3.
@@ -82,55 +66,124 @@ Section ADTValue.
   Import FMapNotations.
   Local Open Scope fmap_scope.
 
+  Arguments SCA {ADTValue} _.
+  Arguments ADT {ADTValue} _.
+
   Require Import ListFacts4.
 
   Require Import Setoid.
+(*
   Add Morphism FRunsTo 
       with signature (@eq FEnv) ==> (@eq Facade.Stmt) ==> (@Equal Value) ==> (@Equal Value) ==> iff as FRunsTo_m.
     admit.
   Qed.
+*)
+
+  Hint Extern 0 (_ == _) => reflexivity.
 
   Require Import StringSet.
 
-  Definition only_diff_in elt (m1 m2 : t elt) s := forall k v1 v2, find k m1 = Some v1 -> find k m2 = Some v2 -> m1 <> m2 -> StringSet.In k s.
+  Definition only_diff_in s (m1 m2 : State) := forall k v1 v2, find k m1 = Some v1 -> find k m2 = Some v2 -> m1 <> m2 -> StringSet.In k s /\ (exists w1, v1 = SCA w1) /\ exists w2, v2 = SCA w2.
 
   Coercion string2elt (x : string) : StringSet.elt := x.
   Coercion StringSet.singleton : StringSet.elt >-> StringSet.t.
 
-  Definition equiv (a b : State) := only_diff_in a b fun_ptr_varname.
+  Definition equiv := only_diff_in fun_ptr_varname.
 
-  Lemma equiv_refl st : equiv st st.
+  Add Morphism equiv 
+      with signature Equal ==> Equal ==> iff as equiv_m.
     admit.
   Qed.
 
+  Infix "===" := equiv (at level 70).
+
   Require Import Option.
 
-  Theorem compile_runsto : 
-    forall t t_env st st', 
-      FRunsTo t_env t st st' -> 
-      forall s, 
-        t = compile s -> 
-        is_syntax_ok s = true -> 
-        forall s_env, 
-          fenv_impls_env t_env s_env -> 
-          Safe s_env s st -> 
+  Lemma is_syntax_ok_seq_elim a b : is_syntax_ok (Seq a b) = true -> is_syntax_ok a = true /\ is_syntax_ok b = true.
+    admit.
+  Qed.
+  Definition is_syntax_ok_e e := StringSet.for_all is_good_varname (FreeVarsExpr.free_vars e).
+  Lemma is_syntax_ok_if_elim e a b : is_syntax_ok (If e a b) = true -> is_syntax_ok_e e = true /\ is_syntax_ok a = true /\ is_syntax_ok b = true.
+    admit.
+  Qed.
+  Lemma is_syntax_ok_while_elim e b : is_syntax_ok (While e b) = true -> is_syntax_ok_e e = true /\ is_syntax_ok b = true.
+    admit.
+  Qed.
+  Lemma is_syntax_ok_assign_elim x e : is_syntax_ok (Assign x e) = true -> is_good_varname x = true /\ is_syntax_ok_e e = true.
+    admit.
+  Qed.
+
+  Lemma find_equiv st1 st2 x : st1 === st2 -> is_good_varname x = true -> find x st1 = find x st2.
+    admit.
+  Qed.
+  Lemma eval_equiv st1 st2 e : st1 === st2 -> is_syntax_ok_e e = true -> eval st1 e = eval st2 e.
+    admit.
+  Qed.
+  Lemma is_false_equiv st1 st2 e : is_false st1 e -> st1 === st2 -> is_syntax_ok_e e = true -> is_false st2 e.
+    admit.
+  Qed.
+  Lemma is_true_equiv st1 st2 e : is_true st1 e -> st1 === st2 -> is_syntax_ok_e e = true -> is_true st2 e.
+    admit.
+  Qed.
+  Lemma not_mapsto_adt_equiv st1 st2 x : st1 === st2 -> is_good_varname x = true -> not_mapsto_adt x st1 = not_mapsto_adt x st2.
+    admit.
+  Qed.
+  Lemma add_equiv st1 st2 x v : st1 === st2 -> is_good_varname x = true -> add x v st1 === add x v st2.
+    admit.
+  Qed.
+
+  Lemma equiv_intro st1 st2 w : st1 == add fun_ptr_varname (SCA w) st2 -> st1 === st2.
+    admit.
+  Qed.
+
+  Lemma equiv_sym a b : a === b -> b === a.
+    admit.
+  Qed.
+
+  Lemma equiv_trans a b c : a === b -> b === c -> a === c.
+    admit.
+  Qed.
+
+  Add Relation State equiv
+      symmetry proved by equiv_sym
+      transitivity proved by equiv_trans
+        as equiv_rel.
+
+  Lemma is_syntax_ok_call_elim x f args : is_syntax_ok (Call x f args) = true -> is_good_varname x = true /\ List.forallb is_good_varname args = true.
+    admit.
+  Qed.
+
+  Lemma mapM_find_equiv st1 st2 ls : st1 === st2 -> List.forallb is_good_varname ls = true -> mapM (sel st1) ls = mapM (sel st2) ls.
+    admit.
+  Qed.
+  Arguments mapM_find_equiv st1 st2 [_] _ _.
+
+  Lemma add_remove_many_equiv st1 st2 args input output : st1 === st2 -> List.forallb is_good_varname args = true -> add_remove_many args input output st1 === add_remove_many args input output st2.
+    admit.
+  Qed.
+
+  Theorem compile_runsto t t_env t_st t_st' :
+    FRunsTo t_env t t_st t_st' -> 
+    forall s, 
+      t = compile s -> 
+      is_syntax_ok s = true -> 
+      forall s_env, 
+        fenv_impls_env t_env s_env -> 
+        forall s_st,
+          Safe s_env s s_st -> 
+          equiv s_st t_st ->
           exists s_st',
-            RunsTo s_env s st s_st' /\
-            equiv s_st' st'. 
+            RunsTo s_env s s_st s_st' /\
+            equiv s_st' t_st'. 
   Proof.
-    induction 1; simpl; destruct s; unfold_all; simpl in *; try solve [intros; try discriminate]; intros Hcomp Hsyn s_env Henv Hsf.
+    induction 1; simpl; destruct s; unfold_all; simpl in *; try solve [intros; try discriminate]; intros Hcomp Hsyn s_env Henv s_st Hsf Heqv.
     {
       (* skip *)
-      exists st.
-      split.
+      exists s_st; split.
       - eapply RunsToSkip; eauto.
-      - eapply equiv_refl; eauto.
+      - eauto.
     }
     {
-      Lemma is_syntax_ok_seq_elim a b : is_syntax_ok (Seq a b) = true -> is_syntax_ok a = true /\ is_syntax_ok b = true.
-        admit.
-      Qed.
-
       (* seq *)
       inject Hcomp.
       inversion Hsf; subst.
@@ -141,21 +194,36 @@ Section ADTValue.
       destruct Hsyn as [Hsyn1 Hsyn2].
       edestruct IHRunsTo1 as [s_st' [Hsst' Heq']]; eauto.
       edestruct IHRunsTo2 as [s_st'' [Hsst'' Heq'']]; eauto.
-      (*here*)
-      eapply Hsf2; eauto.
-      eapply
-      eapply RunsToSeq; eauto.
+      exists s_st''; split.
+      - eapply RunsToSeq; eauto.
+      - eauto.
     }
     {
       (* call *)
       inject Hcomp.
+      rename s into x.
+      rename g into lbl.
+      rename l into args.
       rename H into Hrtlbl.
       rename H0 into Hrtcall.
       inversion Hrtlbl; subst.
       rename H1 into Hlw.
       rename H2 into Hnadt.
       rename H5 into Hst'.
-      rewrite Hst' in Hrtcall.
+      copy_as Hst' Hst'2.
+      eapply equiv_intro in Hst'.
+      assert (Heqv' : st' === s_st) by
+          (etransitivity; eauto; symmetry; eauto).
+      eapply is_syntax_ok_call_elim in Hsyn.
+      destruct Hsyn as [Hsynx Hsynargs].
+      inversion Hsf; subst.
+      rename H2 into Hflbl.
+      rename H3 into Hmm'.
+      rename H5 into Hxnadt.
+      rename H6 into Hpre'.
+      copy_as Hflbl Hflbl'; eapply Henv in Hflbl.
+      destruct Hflbl as [f_w' [Hfw' Hspec']]; simpl in *.
+      unif f_w'.
       inversion Hrtcall; unfold_all; subst.
       {
         (* axiomatic *)
@@ -167,43 +235,107 @@ Section ADTValue.
         rename H8 into Hlen.
         rename H11 into Hpost.
         rename H12 into Hst''.
-        inversion Hsf; subst.
+        simpl in *.
+        rewrite Hst'2 in Hfw.
+        rewrite add_eq_o in Hfw by eauto.
+        inject Hfw.
+        unif (Facade.Axiomatic spec0).
+        rewrite (mapM_find_equiv st' s_st) in Hmm by eauto.
+        unif input0.
+        exists (add x ret (add_remove_many args input (wrap_output output) s_st)).
+        split.
         {
-          eapply RunsToCallAx.
-        
-
+          eapply RunsToCallAx; eauto.
+        }
+        {
+          rewrite Hst''.
+          eapply add_equiv; eauto.
+          eapply add_remove_many_equiv; eauto.
+          symmetry; eauto.
+        }
+      }
+      {
+        (* operational *)
+        rename H3 into Hfw.
+        rename H4 into Hspec.
+        simpl in *.
+        rewrite Hst'2 in Hfw.
+        rewrite add_eq_o in Hfw by eauto.
+        inject Hfw.
+        rewrite Hspec in Hspec'; discriminate.
+      }
     }
     {
       (* if-true *)
       inject Hcomp.
+      eapply is_syntax_ok_if_elim in Hsyn.
+      destruct Hsyn as [Hsyne [Hsyn1 Hsyn2]].
       inversion Hsf; subst; rename H5 into He; rename H6 into Hsfbr.
-      - eapply RunsToIfTrue; eauto.
-      - exfalso; eapply is_true_is_false; eauto.
+      - edestruct IHRunsTo as [s_st' [Hsst' Heq']]; eauto.
+        exists s_st'; split.
+        + eapply RunsToIfTrue; eauto.
+        + eauto.
+      - eapply is_false_equiv in He; eauto.
+        exfalso; eapply is_true_is_false; eauto.
     }
     {
       (* if-false *)
       inject Hcomp.
+      eapply is_syntax_ok_if_elim in Hsyn.
+      destruct Hsyn as [Hsyne [Hsyn1 Hsyn2]].
       inversion Hsf; subst; rename H5 into He; rename H6 into Hsfbr.
-      - exfalso; eapply is_true_is_false; eauto.
-      - eapply RunsToIfFalse; eauto.
+      - eapply is_true_equiv in He; eauto.
+        exfalso; eapply is_true_is_false; eauto.
+      - edestruct IHRunsTo as [s_st' [Hsst' Heq']]; eauto.
+        exists s_st'; split.
+        + eapply RunsToIfFalse; eauto.
+        + eauto.
     }
     {
       (* while-true *)
       inject Hcomp.
+      copy_as Hsyn Hsyn'.
+      eapply is_syntax_ok_while_elim in Hsyn.
+      destruct Hsyn as [Hsyne Hsynb].
       inversion Hsf; unfold_all; subst.
-      - eapply RunsToWhileTrue; eauto.
-      - exfalso; eapply is_true_is_false; eauto.
+      - edestruct IHRunsTo1 as [s_st' [Hsst' Heq']]; eauto.
+        edestruct (IHRunsTo2 (While e s)) as [s_st'' [Hsst'' Heq'']]; try eapply Heq'; eauto.
+        exists s_st''; split.
+        + eapply RunsToWhileTrue; eauto.
+        + eauto.
+      - rename H5 into He.
+        eapply is_false_equiv in He; eauto.
+        exfalso; eapply is_true_is_false; eauto.
     }
     {
       (* while-false *)
       inject Hcomp.
+      eapply is_syntax_ok_while_elim in Hsyn.
+      destruct Hsyn as [Hsyne Hsynb].
       inversion Hsf; unfold_all; subst.
-      - exfalso; eapply is_true_is_false; eauto.
-      - eapply RunsToWhileFalse; eauto.
+      - rename H2 into He.
+        eapply is_true_equiv in He; eauto.
+        exfalso; eapply is_true_is_false; eauto.
+      - exists s_st; split.
+        + eapply RunsToWhileFalse; eauto.
+        + eauto.
     }
     {
       (* assign *)
       inject Hcomp.
-      eapply RunsToAssign; eauto.
+      rename s into x.
+      rename H into He.
+      rename H0 into Hnadt.
+      rename H1 into Hst'.
+      eapply is_syntax_ok_assign_elim in Hsyn.
+      destruct Hsyn as [Hsynx Hsyne].
+      erewrite <- eval_equiv in He by eauto.
+      erewrite <- not_mapsto_adt_equiv in Hnadt by eauto.
+      exists (add x (SCA w) s_st); split.
+      - eapply RunsToAssign; eauto.
+      - rewrite Hst'.
+        eapply add_equiv; eauto.
     }
   Qed.
+
+End ADTValue.
