platform/facade/DFacade.v
@@ -111,11 +111,8 @@ Section ADTSection.
       syntax_ok : is_syntax_ok Body = true
     }.
 
-  Inductive FuncSpec :=
-    | Axiomatic : AxiomaticSpec -> FuncSpec
-    | Operational : OperationalSpec -> FuncSpec.
-
-  Definition Env := GLabelMap.t FuncSpec.
+  (* Only supports axiomatic specs. Don't know how to prove compilation when there are operational specs. *)
+  Definition Env := GLabelMap.t AxiomaticSpec.
 
   Section EnvSection.
 
@@ -160,30 +157,13 @@ Section ADTSection.
           RunsTo (Assign x e) st st'
     | RunsToCallAx :
         forall x f args st spec input output ret,
-          GLabelMap.find f env = Some (Axiomatic spec) ->
+          GLabelMap.find f env = Some spec ->
           mapM (sel st) args = Some input ->
           not_mapsto_adt x st = true ->
           PreCond spec input ->
           length input = length output ->
           PostCond spec (combine input output) ret ->
           let st' := add_remove_many args input (wrap_output output) st in
-          let st' := add x ret st' in
-          forall st'',
-            st'' == st' ->
-            RunsTo (Call x f args) st st''
-    | RunsToCallOp :
-        forall x f args st spec input callee_st' ret,
-          GLabelMap.find f env = Some (Operational spec) ->
-          length args = length (ArgVars spec) ->
-          mapM (sel st) args = Some input ->
-          not_mapsto_adt x st = true ->
-          let callee_st := make_map (ArgVars spec) input in
-          RunsTo (Body spec) callee_st callee_st' ->
-          sel callee_st' (RetVar spec) = Some ret ->
-          (* prevent memory leak *)
-          no_adt_leak input (ArgVars spec) (RetVar spec) callee_st' ->
-          let output := List.map (sel callee_st') (ArgVars spec) in
-          let st' := add_remove_many args input output st in
           let st' := add x ret st' in
           forall st'',
             st'' == st' ->
@@ -227,24 +207,10 @@ Section ADTSection.
           Safe (Assign x e) st
     | SafeCallAx :
         forall x f args st spec input,
-          GLabelMap.find f env = Some (Axiomatic spec) ->
+          GLabelMap.find f env = Some spec ->
           mapM (sel st) args = Some input ->
           not_mapsto_adt x st = true ->
           PreCond spec input ->
-          Safe (Call x f args) st
-    | SafeCallOp :
-        forall x f args st spec input,
-          GLabelMap.find f env = Some (Operational spec) ->
-          length args = length (ArgVars spec) ->
-          mapM (sel st) args = Some input ->
-          not_mapsto_adt x st = true ->
-          let callee_st := make_map (ArgVars spec) input in
-          Safe (Body spec) callee_st ->
-          (* all paths of callee must be memory-leak free and produce a return value *)
-          (forall callee_st', 
-             RunsTo (Body spec) callee_st callee_st' -> 
-             sel callee_st' (RetVar spec) <> None /\ 
-             no_adt_leak input (ArgVars spec) (RetVar spec) callee_st') ->
           Safe (Call x f args) st.
 
     Section Safe_coind.
@@ -275,18 +241,9 @@ Section ADTSection.
           not_mapsto_adt x st = true /\
           exists input, 
             mapM (sel st) args = Some input /\
-            ((exists spec,
-                GLabelMap.find f env = Some (Axiomatic spec) /\
-                PreCond spec input) \/
-             (exists spec,
-                GLabelMap.find f env = Some (Operational spec) /\
-                length args = length (ArgVars spec) /\
-                let callee_st := make_map (ArgVars spec) input in
-                R (Body spec) callee_st /\
-                (forall callee_st',
-                   RunsTo (Body spec) callee_st callee_st' ->
-                   sel callee_st' (RetVar spec) <> None /\
-                   no_adt_leak input (ArgVars spec) (RetVar spec) callee_st'))).
+            exists spec,
+                GLabelMap.find f env = Some spec /\
+                PreCond spec input.
       
       Hint Constructors Safe.
 
